code/ecdsap256sha2/Hacl.Impl.P256.PointDouble.fsti
@@ -9,16 +9,16 @@ open Hacl.Impl.P256.Arithmetics
 
 open Lib.Buffer
 
-open Hacl.Spec.P256.Lemmas
-open Hacl.Spec.P256.Definitions
+open Spec.P256.Lemmas
+open Spec.P256.Definitions
+open Spec.P256.MontgomeryMultiplication
+open Spec.P256.MontgomeryMultiplication.PointDouble
+open Spec.P256.MontgomeryMultiplication.PointAdd
+open Spec.P256
 open Hacl.Impl.SolinasReduction
-open Hacl.Spec.P256.MontgomeryMultiplication
-open Hacl.Spec.P256.MontgomeryMultiplication.PointDouble
-open Hacl.Spec.P256.MontgomeryMultiplication.PointAdd
 open Hacl.Impl.LowLevel
 open Hacl.Impl.P256.LowLevel
 open Hacl.Impl.P256.MontgomeryMultiplication
-open Hacl.Spec.P256
 open Hacl.Impl.P256.Math 
 
 open FStar.Tactics 
